New kripke handler, rewrite rr and bakery

examples/Messaging/Bakery.v
@@ -1,188 +1,97 @@
 From ITree Require Import
-     Basics
      Subevent
-     Events.State
+     CategoryOps
      Indexed.Sum.
 
-From Coq Require Import
-     Fin
-     Nat
-     Vector
-     Logic.Eqdep
-     Classes.RelationClasses
-     Program.Tactics.
-
-From Equations Require Import Equations.
+From Coq Require Import Nat List.
 
 From ExtLib Require Import
-     RelDec
-     Monad
-     Option.
-
-From Coinduction Require Import
-     coinduction rel tactics.
+     Data.Nat
+     Structures.Monad
+     Structures.MonadState
+     Data.Monads.StateMonad
+     Structures.Maps
+     Data.Map.FMapAList.
 
 From CTree Require Import
      CTree
      Eq
-     Interp
-     Interp.State
-     Interp.Log
      Interp.Network
-     Logic.Ltl
-     Misc.Vectors.
+     Logic.Kripke
+     Logic.Ctl.
 
-Import CTreeNotations VectorNotations Log LtlNotations Monads Network CTree.  
-Local Open Scope fin_vector_scope.
+Import MonadNotation CtlNotations.
+Local Open Scope list_scope.
+Local Open Scope monad_scope.
 Local Open Scope ctree_scope.
 
 Set Implicit Arguments.
-Set Maximal Implicit Insertion.
-Set Asymmetric Patterns.
 
-Module Bakery.
-  Section ParametricN.
-    Context {n: nat} {C: Type -> Type} {HasTau: B1 -< C}.
+Variant csE: Type -> Type :=
+  | In_CS: bool -> csE unit.
 
-    Inductive msg :=
-    | GetNumber
-    | CS.
+Definition enter_cs {E C} `{csE -< E}: ctree E C unit :=
+  trigger (In_CS true). 
+Definition exit_cs {E C} `{csE -< E}: ctree E C unit :=
+  trigger (In_CS false). 
 
-    Record agent_row := {
-        in_cs: bool;
-        ticket: option nat;
-        id : uid n
-      }.
-   
-    Notation heap := (nat * vec n agent_row)%type (only parsing).
-    Notation Net := (Net n msg).
-    Notation State := (stateE heap).
-    Notation Sys := (vec n (ctree (Net +' State))).
-    
-    (** ===================================================================== *)
-    (** Lamport's bakery algorithm *)
+#[global] Instance handler_cs: csE ~~> state bool :=
+  fun _ e => match e with
+          | In_CS b => put b
+          end.
 
-    (*| Utility function, find the agent with the earliest (min) issued ticket |*)
-    Equations get_min_ticket'{n: nat}(v: vec n agent_row)(sm: option agent_row): option agent_row :=
-      get_min_ticket' [] _ := sm;
-      get_min_ticket' (h:: ts) None => get_min_ticket' ts (Some h);
-      get_min_ticket' (h :: ts) (Some m) with (h.(ticket), m.(ticket)) => {
-        | (Some ht, Some mt) with ht <? mt => {            
-          | true := get_min_ticket' ts (Some h);
-          | false := get_min_ticket' ts (Some m);
-          };
-        | (None, Some _) := get_min_ticket' ts (Some m);
-        | (Some _, None) := get_min_ticket' ts (Some h);
-        | (None, None) := get_min_ticket' ts None
-        }.
-    Definition get_min_ticket{n: nat}(v: vec n agent_row) := get_min_ticket' v None.
+From CTree Require Import FoldStateT.
 
-    Definition get_agents {E} `{State -< E}: ctree E C (vec n agent_row) :=
-      get >>= fun p => ret (snd p). 
+(*| Client process |*)
+Definition client (id: uid)(bakery: uid): ctree (netE uid +' csE) B1 void :=
+  CTree.forever (
+      (* 1. Ask for a ticket number *)
+      send bakery id;;
+      (* 2. Loop until received [CS] message *)
+      CTree.iter (fun _ =>
+                    m <- recv;;
+                    match m with
+                    | Some x => if x =? bakery then 
+                                 enter_cs;;
+                                 (* DO WORK HERE*)
+                                 exit_cs;;
+                                 Ret (inr tt)
+                               else
+                                 Ret (inl tt)                                 
+                    | None => Ret (inl tt)
+                    end) tt).
 
-    Definition update_agents {E} `{State -< E}(m: agent_row): ctree E C unit :=
-      st <- get;;
-      match st with
-      | (cnt, v) => put (cnt, v @ m.(id) := m)
-      end.
+(* A finite map of [uid] to their number *)
+Notation baker_map := (alist uid nat) (only parsing).
 
-    (*| The baker process, synchronized access to CS through ticket |*)
-    Definition baker: ctree (Net +' State) C void :=
-      daemon (
-          (* 1. Schedule a Critical Section (CS) if possible *)
-          v <- get_agents;;
-          match get_min_ticket v with
-          | None => ret tt
-          | Some st =>
-              send st.(id) CS;; (* Baker sends [CS] msg to preempt clients to enter their CS *)
-              update_agents {| in_cs := true; ticket := None; id := st.(id) |}
-          end;;
-          (* 2. Listen to issue new ticket number *)
-          CTree.iter (fun _: unit =>
-                        m <- recv;;
-                        match m with
-                        | Some (Build_req id GetNumber) =>
-                            st <- get;;
-                            match st with
-                            | (cnt, v) => (* Bump the counter after assigning a ticket to client [id] *)
-                                put (S cnt, v @ id := {| in_cs := false; ticket := Some cnt; id := id |});;
-                                ret (inr tt)
-                            end
-                        | Some (Build_req id CS) => (* Clients respond to the Baker's [CS] with [CS] when done *)
-                            update_agents {| in_cs := false; ticket := None; id := id |};;
-                            ret (inr tt)
-                        | None =>
-                            ret (inl tt)
-                        end) tt).                             
-    
-    (*| Client process |*)
-    Definition client (id: uid n)(bakery: uid n) : ctree (Net +' State) C void :=
-      daemon (
-          (* 1. Ask for a ticket number *)
-          send bakery GetNumber;;
-          (* 2. Loop until received [CS] message *)
-          CTree.iter (fun _: unit =>
-                        m <- recv;;
-                        match m with
-                        | Some (Build_req _ CS) =>
-                            (* ENTER CRITICAL SECTION *)
-                            send bakery CS;;
-                            (* When done send back [CS] to bakery and break inner loop *)
-                            ret (inr tt)
-                        | _ => ret (inl tt) (* Clients refuse to handle [GetNumber] *)
-                        end) tt).
+(* Find the minimum number *)
+Definition alist_minv: baker_map -> option (uid * nat) :=
+  fold_alist (fun k v acc => match acc with
+                          | None => Some (k, v)
+                          | Some (km, vm) => if v <? vm then Some (k, v) else Some (km, vm)
+                          end) None.
 
-    (** ================================================================================ *)
-    (** This is the top-level denotation *)
-    Program Definition run_network_state{C} `{B1 -< C} `{B2 -< C} `{Bn -< C}
-            (v: vec n (ctree (Net +' State) C void)): heap -> ctree (frameE n +' logE heap) C void :=
-      fun st: heap => run_network (run_states_log v st).  
-  End ParametricN.
-End Bakery.
-
-(*| Try out the bakery algorithm with 2 nodes and 1 baker |*)
-Module TestBakery.
-  Import Bakery.
-  
-  (*| First client [A] |*)
-  Program Definition A : uid 3 := @of_nat_lt 0 _ _.
-  (*| Second client [B] |*)
-  Program Definition B : uid 3 := @of_nat_lt 1 _ _.
-  (*| Baker |*)
-  Program Definition bakery: uid 3 := @of_nat_lt 2 _ _.
-  (*| Initial state of the baker, clients are stateless |*)
-  Program Definition init_state :=
-    (0, [
-        {| in_cs := false; ticket := None; id := A |};
-        {| in_cs := false; ticket := None; id := B |};
-        {| in_cs := false; ticket := None; id := bakery |}]).
-
-  (* Now we can generate all schedules for the bakery (slow) *)
-  (* Compute run_network_state [baker; client A bakery; client B bakery] init_state. *)
-  Notation heap := (nat * vec 3 (@agent_row 3))%type (only parsing).
-  Notation Trace := (frameE 3 +' logE heap).
-
-  Arguments label: clear implicits.
-
-  (*| A context switch event predicate -- process [m] is scheduled *)
-  Variant is_in_frame: uid 3 -> label Trace -> Prop :=
-    | ProcessEnter: forall m, is_in_frame m (obs (inl1 (Enter m)) tt).
-  
-  (*| Is a process in their critical section? If yes, then safety property must be satisfied |*)
-  Variant is_in_cs: uid 3 -> label Trace -> Prop :=
-    | ProcessInCs: forall i agents a cnt,
-        (agents $ i).(in_cs) = true ->                       (* [i] is in their CS *)
-        get_min_ticket agents = Some a /\ a.(id) = i ->       (* [i] holds the min ticket *)
-        (forall j, j <> i -> (agents $ j).(in_cs) = false) ->       (* nobody else is in the CS *)
-        is_in_cs i (obs (inr1 (Log (cnt, agents))) tt).
-
-  Lemma correctness_lemma: forall i,
-      let sys :=  run_network_state [baker; client A bakery; client B bakery] init_state in
-      sys |= InfinitelyOften (Spec (is_in_frame i)) ->      (* Axiomatize fairness *)
-      sys |= Eventually (Spec (is_in_cs i)).               (* Liveness + safety *)
-  Proof.
-    (* WIP *)
-  Admitted.
-      
-End TestBakery.
+(*| The baker process, synchronized access to CS through ticket |*)
+Definition baker(bkid: uid): ctree (netE uid +' stateE (nat * baker_map)) B1 void :=
+  CTree.forever (
+      (* 1. Schedule a Critical Section (CS) if possible *)
+      '(cnt, book) <- get ;;
+      match alist_minv book with
+      | None => Ret tt
+      | Some (i, _) =>
+          (* Remove picked user from the queue *)
+          put (cnt, alist_remove _ i book) ;;
+          (* Baker sends his own [bkid] for client [i] to enter CS *)
+          send i bkid 
+      end ;;
+      (* 2. Listen to issue new ticket number *)
+      CTree.iter (fun _: unit =>
+                    m <- recv;;
+                    match m with
+                    | Some id =>
+                        put (S cnt, alist_add _ id cnt book);;
+                        Ret (inr tt)
+                    | None =>
+                        Ret (inl tt)
+                    end) tt).
 
